Hungarian_Method/WBP_Matching_Exec.thy
@@ -1,0 +1,821 @@
+theory WBP_Matching_Exec
+  imports WBP_Matching_Reductions_Exec  "HOL-Library.Product_Lexorder"
+begin
+
+section \<open>Executable Algorithms for Weighted Bipartite Matching\<close>
+
+instantiation bp_vertex_wrapper :: (linorder) linorder
+begin
+
+fun less_eq_bp_vertex_wrapper where
+"less_eq_bp_vertex_wrapper (old_vertex u) (old_vertex v) \<longleftrightarrow> u \<le> v"|
+"less_eq_bp_vertex_wrapper (old_vertex u) (new_vertex i) \<longleftrightarrow> True"|
+"less_eq_bp_vertex_wrapper (new_vertex i) (old_vertex u) \<longleftrightarrow> False"|
+"less_eq_bp_vertex_wrapper (new_vertex i) (new_vertex j) \<longleftrightarrow> i \<le> j"
+
+fun less_bp_vertex_wrapper where
+"less_bp_vertex_wrapper (old_vertex u) (old_vertex v) \<longleftrightarrow> u < v"|
+"less_bp_vertex_wrapper (old_vertex u) (new_vertex i) \<longleftrightarrow> True"|
+"less_bp_vertex_wrapper (new_vertex i) (old_vertex u) \<longleftrightarrow> False"|
+"less_bp_vertex_wrapper (new_vertex i) (new_vertex j) \<longleftrightarrow> i < j"
+
+instance 
+proof(standard, goal_cases)
+  case (1 x y)
+  then show ?case
+    by(cases x, all \<open>cases y\<close>) auto
+next
+  case (2 x)
+  then show ?case 
+   by(cases x) auto
+next
+  case (3 x y z)
+  then show ?case 
+   by(cases x, all \<open>cases y\<close>, all \<open>cases z\<close>) auto
+next
+  case (4 x y)
+  then show ?case
+   by(cases x, all \<open>cases y\<close>) auto
+next
+  case (5 x y)
+  then show ?case 
+   by(cases x, all \<open>cases y\<close>) auto
+qed
+
+end
+
+lemma trivial_map: "Map (\<lambda>x. None) (\<lambda>x y f. f(x \<mapsto> y)) (\<lambda>x f. f(x := None)) (\<lambda>f. f) (\<lambda>f. True)"
+  by(auto intro!: Map.intro)
+
+global_interpretation graph_completer_spec_rbt: graph_completer_spec
+  where delete = delete
+  and lookup = lookup
+  and isin = isin
+  and t_set = t_set
+  and sel = sel
+  and update = update
+  and adjmap_inv= M.invar
+  and vset_delete = vset_delete
+  and vset_inv = vset_inv
+  and empty = map_empty
+  and vset_empty = vset_empty
+  and insert = vset_insert
+  and oempty = "\<lambda> x. None"
+  and odelete = "\<lambda> x f. fun_upd f x None"
+  and olookup = "\<lambda> f x. f x"
+  and oinsert = vset_insert
+  and oisin = isin
+  and ot_set = t_set
+  and osel = sel
+  and oupdate =  "\<lambda> x y f. fun_upd f x (Some y)"
+  and oadjmap_inv="\<lambda> f. True"
+  and ovset_empty = vset_empty
+  and ovset_delete = vset_delete
+  and ovset_inv = vset_inv
+  and ovset_fold_reals = "\<lambda> f T x. rbt_set_fold T f x"
+  and cempty = Leaf
+  and cupdate = update
+  and cdelete = delete
+  and clookup = lookup
+  and cinvar = M.invar
+  and obempty = Leaf
+  and obupdate = update
+  and obdelete= delete
+  and oblookup=lookup
+  and obinvar =M.invar
+  and bempty="\<lambda> x. None"
+  and bupdate= "\<lambda> x y f. fun_upd f x (Some y)"
+  and bdelete= "\<lambda> x f. fun_upd f x None"
+  and blookup= "\<lambda> f x. f x"
+  and binvar = "\<lambda> f. True"
+  and vset_to_list = "inorder"
+  and left = left
+  and right = right
+  and Gimpl = Gimpl
+  and edge_costs = edge_costs
+for left right Gimpl edge_costs
+defines lsize=graph_completer_spec_rbt.lsize
+and rsize = graph_completer_spec_rbt.rsize
+and new_left_list = graph_completer_spec_rbt.new_left_list
+and new_right_list = graph_completer_spec_rbt.new_right_list
+and new_edge_list = graph_completer_spec_rbt.new_edge_list
+and bp_perfect_exec = graph_completer_spec_rbt.bp_perfected_exec
+and new_left = graph_completer_spec_rbt.new_left
+and new_right = graph_completer_spec_rbt.new_right
+and max_abs_weight = graph_completer_spec_rbt.max_abs_weight
+and penalty_exec = graph_completer_spec_rbt.penalty_exec
+and new_costs_mcst = graph_completer_spec_rbt.new_costs_mcst
+and bp_min_costs_to_min_perfect_costs_exec = graph_completer_spec_rbt.bp_min_costs_to_min_perfect_costs_exec
+and new_costs_mcmc = graph_completer_spec_rbt.new_costs_mcmc
+and bp_min_max_card_costs_to_min_perfect_costs_exec = graph_completer_spec_rbt.bp_min_max_card_costs_to_min_perfect_costs_exec
+and extract_mw_matching= graph_completer_spec_rbt.extract_mw_matching
+and extract_mwmc_matching=graph_completer_spec_rbt.extract_mwmc_matching
+and add_edge = graph_completer_spec_rbt.new_graph.add_edge
+and oheighbourhood=graph_completer_spec_rbt.old_graph.neighbourhood
+and from_list = graph_completer_spec_rbt.new_graph.from_list
+proof(rule graph_completer_spec.intro, goal_cases)
+  case 1
+  then show ?case 
+    by(auto intro!: Pair_Graph_Specs.intro 
+          simp add: Map_axioms_as_needed map_empty_def RBT_Set.empty_def S_C.Set_Choose_axioms)
+next
+  case 2
+  then show ?case 
+    by(auto intro!: Pair_Graph_Specs.intro trivial_map
+          simp add: RBT_Set.empty_def S_C.Set_Choose_axioms)
+next
+  case 3
+  then show ?case
+  proof(rule Set_Iterable.intro, goal_cases)
+    case (1 S f acc)
+    then show ?case 
+    using rbt_set_fold_correct[of S f acc] 
+    by(auto simp add: vset_inv_def t_inv_def) 
+qed
+next
+  case 4
+  then show ?case 
+    by (simp add: pd_path_search_spec.missed_map.Map_axioms)
+next
+  case 6
+  then show ?case 
+    by (simp add: aug_a_matching.buddy_map.Map_axioms)
+next
+  case 5
+  then show ?case 
+    by(simp add: trivial_map)
+qed
+
+(*TODO MOVE*)
+interpretation map_iterator_rbt: Map_iterator M.invar lookup update_all
+  using update_all
+  by(fastforce intro!: Map_iterator.intro update_all
+             simp add: M.invar_def RBT_Set.rbt_def domI rbt_red_def update_all(1)
+                       color_no_change)
+
+global_interpretation invert_costs: cost_inverter
+  where invar = M.invar
+  and update_all = update_all
+  and lookup = lookup
+defines inverted_costs = invert_costs.inverted_costs
+  using update_all
+  by(auto intro!: cost_inverter.intro map_iterator_rbt.Map_iterator_axioms)
+
+hide_const right
+
+definition "compute_min_weight_perfect_matching left right edge_costs right_neighbs
+    = hungarian left right edge_costs right_neighbs lookup RBT_Map.update"
+
+definition "compute_max_weight_perfect_matching left right edge_costs right_neighbs
+         = compute_min_weight_perfect_matching left right (- edge_costs) right_neighbs"
+
+definition "compute_max_weight_perfect_matching_inv left right edge_costs right_neighbs
+         = compute_min_weight_perfect_matching left right 
+            (curry (abstract_real_map (lookup (inverted_costs edge_costs)))) right_neighbs"
+
+definition "acompute_min_matching left right edge_costs right_neighbs
+            = the (
+                compute_min_weight_perfect_matching
+                (new_left left right) 
+                (new_right left right)
+                (curry (abstract_real_map (lookup 
+                      (bp_min_costs_to_min_perfect_costs_exec 
+                           left right right_neighbs edge_costs))))
+                 (lookup (bp_perfect_exec left right)))"
+
+definition "compute_min_weight_matching left right edge_costs right_neighbs
+            = extract_mw_matching left right_neighbs edge_costs
+               (lookup (acompute_min_matching left right edge_costs right_neighbs))"
+
+definition "compute_max_weight_matching left right edge_costs right_neighbs
+         = compute_min_weight_matching left right (- edge_costs) right_neighbs"
+
+definition "compute_max_weight_matching_inv left right edge_costs right_neighbs
+         = compute_min_weight_matching left right 
+            (curry (abstract_real_map (lookup (inverted_costs edge_costs)))) right_neighbs"
+
+definition "acompute_min_max_matching left right edge_costs right_neighbs
+            = the (
+                compute_min_weight_perfect_matching 
+                (new_left left right) 
+                (new_right left right)
+                (curry (abstract_real_map (lookup 
+                      (bp_min_max_card_costs_to_min_perfect_costs_exec 
+                           left right right_neighbs edge_costs))))
+                 (lookup (bp_perfect_exec left right)))"
+
+definition "compute_min_weight_max_card_matching left right edge_costs right_neighbs
+            = extract_mwmc_matching left right_neighbs
+               (lookup (acompute_min_max_matching left right edge_costs right_neighbs))"
+
+definition "compute_max_weight_max_card_matching left right edge_costs right_neighbs
+         = compute_min_weight_max_card_matching left right (- edge_costs) right_neighbs"
+
+definition "compute_max_weight_max_card_matching_inv left right edge_costs right_neighbs
+         = compute_min_weight_max_card_matching left right 
+            (curry (abstract_real_map (lookup (inverted_costs edge_costs)))) right_neighbs"
+
+locale bp_min_weight_matching_algorithms_correct = 
+  fixes G::"('v::linorder) set set"
+    and edge_costs::"'v \<Rightarrow> 'v \<Rightarrow> real"
+    and left::"('v \<times> color) tree"
+    and right::"('v \<times> color) tree"
+    and right_neighbs::"'v \<Rightarrow> (('v \<times> color) tree) option"
+
+assumes G: "bipartite G (vset_to_set left) (vset_to_set right)"
+  "vset_inv left" "vset_inv right"
+  "(vset_to_set left) \<union> (vset_to_set right) \<subseteq> Vs G"
+
+"\<And> v N. \<lbrakk>v \<in> vset_to_set left;right_neighbs v= Some N\<rbrakk> 
+                 \<Longrightarrow> vset_inv N"
+"\<And> v .  v \<in> vset_to_set left 
+                     \<Longrightarrow> \<exists> N .right_neighbs v= Some N \<and>
+                            vset_to_set N = {u | u. {v, u} \<in> G}"
+"\<And> u v. {u, v} \<in> G \<Longrightarrow> edge_costs u v = edge_costs v u"
+begin
+
+abbreviation "\<w> \<equiv> setify_weight edge_costs"
+
+interpretation graph_completer_min: graph_completer
+  where delete = delete
+  and lookup = lookup
+  and isin = isin
+  and t_set = t_set
+  and sel = sel
+  and update = update
+  and adjmap_inv= M.invar
+  and vset_delete = vset_delete
+  and vset_inv = vset_inv
+  and empty = map_empty
+  and vset_empty = vset_empty
+  and insert = vset_insert
+  and oempty = "\<lambda> x. None"
+  and odelete = "\<lambda> x f. fun_upd f x None"
+  and olookup = "\<lambda> f x. f x"
+  and oinsert = vset_insert
+  and oisin = isin
+  and ot_set = t_set
+  and osel = sel
+  and oupdate =  "\<lambda> x y f. fun_upd f x (Some y)"
+  and oadjmap_inv="\<lambda> f. True"
+  and ovset_empty = vset_empty
+  and ovset_delete = vset_delete
+  and ovset_inv = vset_inv
+  and ovset_fold_reals = "\<lambda> f T x. rbt_set_fold T f x"
+  and cempty = Leaf
+  and cupdate = update
+  and cdelete = delete
+  and clookup = lookup
+  and cinvar = M.invar
+  and obempty = Leaf
+  and obupdate = update
+  and obdelete= delete
+  and oblookup=lookup
+  and obinvar =M.invar
+  and bempty="\<lambda> x. None"
+  and bupdate= "\<lambda> x y f. fun_upd f x (Some y)"
+  and bdelete= "\<lambda> x f. fun_upd f x None"
+  and blookup= "\<lambda> f x. f x"
+  and binvar = "\<lambda> f. True"
+  and vset_to_list = "inorder"
+  and left = left
+  and right = right
+  and Gimpl = right_neighbs
+  and edge_costs = some_edge_costs for some_edge_costs
+proof(rule graph_completer.intro, goal_cases)
+  case 1
+  then show ?case 
+proof(rule graph_completer_spec.intro, goal_cases)
+  case 1
+  then show ?case 
+    by(auto intro!: Pair_Graph_Specs.intro 
+          simp add: Map_axioms_as_needed map_empty_def RBT_Set.empty_def S_C.Set_Choose_axioms)
+next
+  case 2
+  then show ?case 
+    by(auto intro!: Pair_Graph_Specs.intro trivial_map
+          simp add: RBT_Set.empty_def S_C.Set_Choose_axioms)
+next
+  case 3
+  then show ?case
+  proof(rule Set_Iterable.intro, goal_cases)
+    case (1 S f acc)
+    then show ?case 
+    using rbt_set_fold_correct[of S f acc] 
+    by(auto simp add: vset_inv_def t_inv_def) 
+qed
+next
+  case 4
+  then show ?case 
+    by (simp add: pd_path_search_spec.missed_map.Map_axioms)
+next
+  case 6
+  then show ?case 
+    by (simp add: aug_a_matching.buddy_map.Map_axioms)
+next
+  case 5
+  then show ?case 
+    by(simp add: trivial_map)
+qed
+next
+  case 2
+  then show ?case
+  proof(rule graph_completer_axioms.intro, goal_cases)
+    case (1 V)
+    then show ?case
+      by (simp add: bst_distinct_inorder vset_inv_def)
+  next
+    case 5
+    then show ?case 
+    proof(rule, all \<open>rule\<close>, goal_cases)
+      case (1 e)
+      then obtain x y where e:"e = {x, y}" "x \<in> (vset_to_set left)" "y \<in>(vset_to_set right)"
+        using G(1) by(auto elim!: bipartite_edgeE)
+      moreover hence "
+          right_neighbs x = Some x2 \<Longrightarrow> graph_completer_spec_rbt.old_graph.isin' y x2" for x2
+       using "1" by(subst RBT.set_isin)(auto dest: G(6) G(5) simp add:  RBT.set_isin vset_inv_def)
+     ultimately have "(x, y) \<in> graph_completer_spec_rbt.old_graph.digraph_abs right_neighbs" 
+        by(auto simp add: graph_completer_spec_rbt.old_graph.digraph_abs_def oheighbourhood_def
+                          Pair_Graph_Specs.neighbourhood_def[OF 
+                            graph_completer_spec_rbt.old_graph.Pair_Graph_Specs_axioms]
+                    dest: G(6)
+                   split: option.split)
+      thus ?case
+        using e by auto
+    next
+      case (2 e)
+      then obtain u v where e:"e = {u, v}" "u \<in> vset_to_set left"
+        "(u, v) \<in> graph_completer_spec_rbt.old_graph.digraph_abs right_neighbs"
+        by auto
+      then obtain N where N: "right_neighbs u = Some N" "vset_to_set N = {ua | ua. {u, ua} \<in> G}"
+        using G(6)[of u] by auto
+      moreover have "graph_completer_spec_rbt.old_graph.isin' v N \<Longrightarrow>
+             v \<in> vset_to_set N"
+        using N(1) e(2) 
+        by(subst (asm) RBT.set_isin)(auto dest: G(5) simp add: vset_inv_def)
+      moreover hence "v \<in> vset_to_set N"
+        using e
+        by(auto simp add: graph_completer_spec_rbt.old_graph.digraph_abs_def
+                          oheighbourhood_def N(1)
+                           Pair_Graph_Specs.neighbourhood_def[OF 
+                            graph_completer_spec_rbt.old_graph.Pair_Graph_Specs_axioms])
+     ultimately show ?case 
+        using e by simp
+    qed     
+  next
+    case 8
+    then show ?case 
+      by(auto intro: graph_completer_spec_rbt.old_graph.finite_vsetsI)
+  next
+    case 9
+    then show ?case 
+      using G(4) by auto
+  qed (simp add: G(1-5))+
+qed
+
+interpretation hungarian_same_graph:
+  hungarian_method_together_correct G some_edge_costs left right  right_neighbs
+  for some_edge_costs
+proof(rule hungarian_method_together_correct.intro, goal_cases)
+  case (5 v N)
+  then show ?case 
+    using graph_completer_min.G(3) by presburger
+next
+  case (6 v)
+  then show ?case
+    using G(6) by auto
+next
+  case 4
+  show ?case
+    using G(4) by auto
+qed (simp add: G(1-3))+
+
+lemmas hungarian_same_graph_correct =
+  hungarian_same_graph.hungarian_correctness[of edge_costs, OF G(7), simplified]
+
+abbreviation "left' \<equiv> new_left left right"
+abbreviation "right' \<equiv> new_right left right"
+abbreviation "right_neighbs' \<equiv> lookup (bp_perfect_exec left right)"
+
+abbreviation "G' \<equiv> bp_perfected_G (vset_to_set left) (vset_to_set right)"
+
+lemma completer_R_left_def: "graph_completer_spec_rbt.R left = vset_to_set left"
+and completer_R_right_def: "graph_completer_spec_rbt.R right = vset_to_set right"
+  by simp+
+
+lemma bipartite_G': "bipartite G' (vset_to_set left') (vset_to_set right')"
+  using graph_completer_min.bipartite_perfected
+      graph_completer_min.bp_perfected_exec_correct(5,7)
+  by(simp add: new_left_def new_right_def)
+
+lemma bp_perfected_L_is_left':
+      "bp_perfected_L (vset_to_set left) (vset_to_set right)= vset_to_set left'"
+and bp_perfected_R_is_right':
+      "bp_perfected_R (vset_to_set left) (vset_to_set right)= vset_to_set right'"
+ by (simp add: graph_completer_min.bp_perfected_exec_correct(5,7) new_left_def new_right_def)+
+
+interpretation hungarian_extended_graph:
+  hungarian_method_together_correct G' some_edge_costs left' right'  right_neighbs'
+  for some_edge_costs
+proof(rule hungarian_method_together_correct.intro, goal_cases)
+  case 1
+  then show ?case 
+    using  graph_completer_min.bipartite_perfected
+        graph_completer_min.bp_perfected_exec_correct(5,7) 
+    by(auto simp add: new_left_def new_right_def)
+next
+  case 2
+  then show ?case 
+    by (simp add: graph_completer_min.bp_perfected_exec_correct(6) new_left_def)
+next
+  case 3
+  then show ?case
+    by (simp add: graph_completer_min.bp_perfected_exec_correct(8) new_right_def)
+next
+  case 4
+  then show ?case 
+    using G(4)
+    by(subst bipartite_Vs_of_complete_union_L_R[of G])
+      (simp add: hungarian_same_graph.G(1) bp_perfected_L_is_left' bp_perfected_R_is_right')+
+next
+  case (5 v N)
+  then show ?case 
+    using  graph_completer_min.bp_perfected_exec_correct(1)
+    by(auto simp add: bp_perfect_exec_def )
+next
+  case (6 v)
+  obtain N where N: "right_neighbs' v = Some N" 
+    using  "6" graph_completer_min.lefts_have_neighb_set
+    by(force simp add: graph_completer_spec_rbt.new_graph.has_neighb_set_def
+               completer_R_left_def
+        completer_R_right_def bp_perfect_exec_def bp_perfected_L_is_left') 
+  hence neighv_is:"N = graph_completer_spec_rbt.new_graph.neighbourhood
+                     (graph_completer_spec.bp_perfected_exec lookup RBT_Map.update map_empty
+                       vset_empty vset_insert left right Tree2.inorder)
+                     v"
+    by(auto simp add: graph_completer_spec_rbt.new_graph.neighbourhood_def bp_perfect_exec_def)
+  have set_ok: "vset_to_set N = { u | u . {v, u} \<in> G'}"
+    unfolding graph_completer_min.bp_perfected_exec_correct(4)[simplified, symmetric]
+              graph_completer_spec_rbt.new_graph.digraph_abs_def 
+  proof(rule, all \<open>rule\<close>, goal_cases)
+    case (1 u)
+    then show ?case 
+      using  graph_completer_spec_rbt.new_graph.are_connected_abs[OF
+              graph_completer_min.bp_perfected_exec_correct(1), of u v]
+      by (auto intro!: in_UDI[of v u] 
+             simp add: neighv_is N forest_manipulation_spec_i.vset.set_isin
+          graph_completer_min.bp_perfected_exec_correct(1))
+  next
+    case (2 u)
+    let ?nbhd = "graph_completer_spec_rbt.new_graph.neighbourhood
+                      (graph_completer_spec.bp_perfected_exec lookup RBT_Map.update map_empty
+                        vset_empty vset_insert left right Tree2.inorder) "
+    have uv_UD:"{v, u} \<in> UD {(u, v) | u v. isin (?nbhd u) v}"
+      using 2 by auto
+    show ?case 
+    proof(cases rule: in_UDE[OF uv_UD])
+      case 1
+      then show ?thesis 
+        by (simp add: forest_manipulation_spec_i.vset.set_isin
+            graph_completer_min.bp_perfected_exec_correct(1) neighv_is)
+    next
+      case 2
+      hence "isin (?nbhd u) v" by force
+      hence "(u, v) \<in> set (graph_completer_spec.new_edge_list left right Tree2.inorder)"
+        using forest_manipulation_spec_i.vset.set_isin graph_completer_min.bp_perfected_exec_correct(1)
+          graph_completer_min.directed_perfected graph_completer_min.new_edge_list_is by blast
+      hence "v \<in> (vset_to_set right')"
+        using graph_completer_min.bp_perfected_exec_correct(7) 
+            graph_completer_min.in_new_edgesE
+        by(simp add: new_right_def)
+      hence False 
+        using "6" bipartite_G' by(auto simp add: bipartite_def)
+      then show ?thesis 
+        by simp
+    qed
+  qed
+  thus ?case 
+    using N by auto
+qed
+
+lemmas hungarian_other_graph_correct = 
+hungarian_extended_graph.hungarian_correctness
+
+lemma compute_min_weight_perfect_matching_correct:
+"compute_min_weight_perfect_matching left right edge_costs right_neighbs = None
+  \<Longrightarrow> \<nexists> M. perfect_matching G M"
+"compute_min_weight_perfect_matching left right edge_costs right_neighbs = Some M
+  \<Longrightarrow> min_weight_perfect_matching G \<w> (matching_abstract M)"
+  using hungarian_same_graph_correct
+   by(auto simp add: compute_min_weight_perfect_matching_def)
+
+(*TODO MOVE*)
+lemma upairs_matching_abstract:
+ "upairs_of_map (lookup M) = matching_abstract M"
+  by(auto simp add: upairs_of_map_def matching_abstract_def
+ matching_augmentation_spec.\<M>_def'[OF aug_a_matching.matching_augmentation_spec_axioms])
+
+lemma extract_mw_matching_same:
+      "graph_completer_spec.extract_mw_matching (\<lambda>f. f) isin vset_empty (\<lambda>f. f) \<langle>\<rangle> RBT_Map.update
+       left edge_costs Tree2.inorder right_neighbs =
+       extract_mw_matching left right_neighbs edge_costs"
+  by(auto simp add: extract_mw_matching_def)
+
+abbreviation "min_weights_used == (curry (abstract_real_map (lookup 
+                      (bp_min_costs_to_min_perfect_costs_exec 
+                           left right right_neighbs edge_costs))))"
+
+lemma weights_used_symmetric:
+  assumes "{u, v} \<in> G'"
+  shows "min_weights_used u v = min_weights_used v u"
+  using G(7)  assms 
+      graph_completer_min.bp_min_costs_to_min_perfect_costs_exec_correct(3)[of edge_costs]
+  by(auto simp add: bp_min_costs_to_min_perfect_costs_exec_def)
+
+lemma balanced_complete_bipartite_G':
+ "balanced_complete_bipartite G' (vset_to_set left') (vset_to_set right')"
+  using  bp_perfected_L_is_left' bp_perfected_R_is_right'
+         graph_completer_min.bp_perfected_props(1) by auto
+
+lemma finite_G': "finite G'"
+  using finite_G' hungarian_same_graph.G(1) by fastforce
+
+lemma hungarian_min_not_None:
+  "hungarian left' right' min_weights_used right_neighbs' lookup RBT_Map.update \<noteq> None"
+  apply(rule ccontr)
+  using perfect_matching_in_balanced_complete_bipartite[OF balanced_complete_bipartite_G' finite_G']
+  by(auto dest!: hungarian_other_graph_correct(1)[of
+         min_weights_used, OF weights_used_symmetric, simplified])
+
+lemma hungarian_min_is_Some:
+    "hungarian left' right' min_weights_used right_neighbs' lookup RBT_Map.update =
+    Some (acompute_min_matching left right edge_costs right_neighbs)"
+  by(auto simp add: acompute_min_matching_def
+    compute_min_weight_perfect_matching_def hungarian_min_not_None)
+
+lemma compute_min_weight_correct:
+"min_weight_matching G \<w> (matching_abstract
+      (compute_min_weight_matching left right edge_costs right_neighbs))"
+proof-
+  note proof_rule = back_subst[of "min_weight_matching _ _", OF
+    graph_completer_min.minimum_weight_matching[of edge_costs,
+    simplified graph_completer_min.\<w>_def, simplified upairs_matching_abstract
+               extract_mw_matching_same], OF _ _ _  refl]
+  show ?thesis
+  unfolding compute_min_weight_matching_def
+proof(rule proof_rule, goal_cases)
+  case (1 u v)
+  then show ?case 
+    using G(7) by blast
+next
+  case (2 u v)
+  then show ?case 
+  proof(rule hungarian_extended_graph.hungarian_symmetric[of min_weights_used],
+         unfold bp_min_costs_to_min_perfect_costs_exec_def,
+       rule graph_completer_min.bp_min_costs_to_min_perfect_costs_exec_correct(3), goal_cases)
+    case (1 u v ua va)
+    then show ?case 
+      using G(7) by auto
+  next
+    case (2 u v)
+    then show ?case
+      by simp
+  next
+    case 3
+    then show ?case 
+      using  hungarian_min_is_Some
+      by(auto simp add: acompute_min_matching_def
+                        bp_min_costs_to_min_perfect_costs_exec_def)
+  qed
+next
+  case 3
+  then show ?case 
+    using  hungarian_min_is_Some
+      hungarian_other_graph_correct(2)[of min_weights_used
+        "acompute_min_matching left right edge_costs right_neighbs",
+                OF weights_used_symmetric, simplified]
+    by(auto simp add: upairs_matching_abstract bp_min_costs_to_min_perfect_costs_exec_def)
+qed
+qed
+
+lemma extract_mwmc_matching_same:
+      "graph_completer_spec.extract_mwmc_matching (\<lambda>f. f) isin vset_empty (\<lambda>f. f) \<langle>\<rangle> RBT_Map.update
+       left  Tree2.inorder right_neighbs =
+       extract_mwmc_matching left right_neighbs"
+  by(auto simp add: extract_mwmc_matching_def)
+
+abbreviation "min_max_card_weights_used == (curry (abstract_real_map (lookup 
+                      (bp_min_max_card_costs_to_min_perfect_costs_exec 
+                           left right right_neighbs edge_costs))))"
+
+lemma max_card_weights_used_symmetric:
+  assumes "{u, v} \<in> G'"
+  shows "min_max_card_weights_used u v = min_max_card_weights_used v u"
+  using G(7)  assms 
+      graph_completer_min.bp_min_max_card_to_min_perfect_costs_exec_correct(3)[of edge_costs]
+  by(auto simp add: bp_min_max_card_costs_to_min_perfect_costs_exec_def)
+
+lemma hungarian_min_max_card_not_None:
+  "hungarian left' right' min_max_card_weights_used right_neighbs' lookup RBT_Map.update \<noteq> None"
+  apply(rule ccontr)
+  using perfect_matching_in_balanced_complete_bipartite[OF balanced_complete_bipartite_G' finite_G']
+  by(auto dest!: hungarian_other_graph_correct(1)[of
+         min_max_card_weights_used, OF max_card_weights_used_symmetric, simplified])
+
+lemma hungarian_min_max_card_is_Some:
+    "hungarian left' right' min_max_card_weights_used right_neighbs' lookup RBT_Map.update =
+    Some (acompute_min_max_matching left right edge_costs right_neighbs)"
+ by(auto simp add: acompute_min_max_matching_def
+    compute_min_weight_perfect_matching_def hungarian_min_max_card_not_None)
+
+lemma compute_min_weight_max_card_correct:
+  "min_weight_max_card_matching G \<w> (matching_abstract
+      (compute_min_weight_max_card_matching left right edge_costs right_neighbs))"
+proof-
+  note proof_rule =  back_subst[of "min_weight_max_card_matching _ _", OF
+    graph_completer_min.minimum_weight_max_card_matching[of edge_costs,
+    simplified graph_completer_min.\<w>_def, simplified upairs_matching_abstract
+               extract_mwmc_matching_same], OF _ _ _  refl]
+  show ?thesis
+  unfolding compute_min_weight_max_card_matching_def
+proof(rule proof_rule, goal_cases)
+  case (1 u v)
+  then show ?case 
+    using G(7) by blast
+next
+  case (2 u v)
+  then show ?case 
+  proof(rule hungarian_extended_graph.hungarian_symmetric[
+            of min_max_card_weights_used],
+         unfold bp_min_max_card_costs_to_min_perfect_costs_exec_def,
+       rule graph_completer_min.bp_min_max_card_to_min_perfect_costs_exec_correct(3), goal_cases)
+    case (1 u v ua va)
+    then show ?case 
+      using G(7) by auto
+  next
+    case (2 u v)
+    then show ?case
+      by simp
+  next
+    case 3
+    then show ?case 
+      using  hungarian_min_max_card_is_Some
+      by(auto simp add: acompute_min_max_matching_def
+                        bp_min_max_card_costs_to_min_perfect_costs_exec_def)
+  qed
+next
+  case 3
+  then show ?case 
+    using  hungarian_min_max_card_is_Some
+      hungarian_other_graph_correct(2)[of min_max_card_weights_used
+        "acompute_min_max_matching left right edge_costs right_neighbs",
+                OF max_card_weights_used_symmetric, simplified]
+    by(auto simp add: upairs_matching_abstract
+                      bp_min_max_card_costs_to_min_perfect_costs_exec_def)
+qed
+qed
+
+lemmas minimum_weight_matching_algos_correct = 
+  compute_min_weight_perfect_matching_correct
+  compute_min_weight_correct
+  compute_min_weight_max_card_correct
+
+end
+
+locale bp_matching_algorithms_correct = 
+  fixes G::"('v::linorder) set set"
+    and edge_costs::"'v \<Rightarrow> 'v \<Rightarrow> real"
+    and left::"('v \<times> color) tree"
+    and right::"('v \<times> color) tree"
+    and right_neighbs::"'v \<Rightarrow> (('v \<times> color) tree) option"
+
+assumes G: "bipartite G (vset_to_set left) (vset_to_set right)"
+  "vset_inv left" "vset_inv right"
+  "(vset_to_set left) \<union> (vset_to_set right) \<subseteq> Vs G"
+
+"\<And> v N. \<lbrakk>v \<in> vset_to_set left;right_neighbs v= Some N\<rbrakk> 
+                 \<Longrightarrow> vset_inv N"
+"\<And> v .  v \<in> vset_to_set left 
+                     \<Longrightarrow> \<exists> N .right_neighbs v= Some N \<and>
+                            vset_to_set N = {u | u. {v, u} \<in> G}"
+"\<And> u v. {u, v} \<in> G \<Longrightarrow> edge_costs u v = edge_costs v u"
+begin
+
+abbreviation "\<w> \<equiv> setify_weight edge_costs"
+
+interpretation min_version:
+  bp_min_weight_matching_algorithms_correct
+  G edge_costs left right right_neighbs
+  using G(1-6)
+  by(auto intro!: bp_min_weight_matching_algorithms_correct.intro dest: G(7))
+
+interpretation max_version:
+  bp_min_weight_matching_algorithms_correct
+  G "- edge_costs" left right right_neighbs
+  using G(1-6)
+  by(auto intro!: bp_min_weight_matching_algorithms_correct.intro dest: G(7))
+
+lemma minus_minus_w: "- (\<lambda>e. - min_version.\<w> e) = \<w>" 
+  by auto
+
+lemma compute_max_weight_perfect_matching_correct:
+"compute_max_weight_perfect_matching left right edge_costs right_neighbs = None
+  \<Longrightarrow> \<nexists> M. perfect_matching G M"
+"compute_max_weight_perfect_matching left right edge_costs right_neighbs = Some M
+  \<Longrightarrow> max_weight_perfect_matching G \<w> (matching_abstract M)"
+  using max_version.minimum_weight_matching_algos_correct(1,2)
+  by(auto simp add: compute_max_weight_perfect_matching_def
+                    min_perfect_and_max_perfect_matching minus_minus_w)
+
+lemma compute_max_weight_correct:
+"max_weight_matching G \<w> (matching_abstract
+      (compute_max_weight_matching left right edge_costs right_neighbs))"
+  using max_version.minimum_weight_matching_algos_correct(3)
+  by(auto simp add: compute_max_weight_matching_def
+                    min_and_max_matching minus_minus_w)
+
+lemma compute_max_weight_max_card_correct:
+  "max_weight_max_card_matching G \<w> (matching_abstract
+      (compute_max_weight_max_card_matching left right edge_costs right_neighbs))"
+  using max_version.minimum_weight_matching_algos_correct(4)
+  by(auto simp add: compute_max_weight_max_card_matching_def
+                    min_max_card_and_max_max_card_matching  minus_minus_w)
+
+lemmas bp_weighted_matching_algos_correct =
+ min_version.minimum_weight_matching_algos_correct
+ compute_max_weight_perfect_matching_correct
+ compute_max_weight_correct
+ compute_max_weight_max_card_correct
+end
+
+locale bp_matching_algorithms_correct_cost_map = 
+  fixes G::"('v::linorder) set set"
+    and edge_costs::"((('v \<times> 'v) \<times> real) \<times> color) tree"
+    and left::"('v \<times> color) tree"
+    and right::"('v \<times> color) tree"
+    and right_neighbs::"'v \<Rightarrow> (('v \<times> color) tree) option"
+
+assumes G: "bipartite G (vset_to_set left) (vset_to_set right)"
+  "vset_inv left" "vset_inv right"
+  "(vset_to_set left) \<union> (vset_to_set right) \<subseteq> Vs G"
+
+"\<And> v N. \<lbrakk>v \<in> vset_to_set left;right_neighbs v= Some N\<rbrakk> 
+                 \<Longrightarrow> vset_inv N"
+"\<And> v .  v \<in> vset_to_set left 
+                     \<Longrightarrow> \<exists> N .right_neighbs v= Some N \<and>
+                            vset_to_set N = {u | u. {v, u} \<in> G}"
+"\<And> u v. {u, v} \<in> G \<Longrightarrow> \<Parallel>lookup edge_costs\<Parallel> (u, v) =  \<Parallel>lookup edge_costs\<Parallel> (v, u)"
+"M.invar edge_costs"
+begin
+
+abbreviation "\<w> \<equiv> setify_weight (curry \<Parallel>lookup edge_costs\<Parallel>)"
+
+interpretation min_version:
+  bp_min_weight_matching_algorithms_correct
+  G "curry \<Parallel>lookup edge_costs\<Parallel>" left right right_neighbs
+  using G(1-6)
+  by(auto intro!: bp_min_weight_matching_algorithms_correct.intro dest: G(7))
+
+lemmas inverted_costs = invert_costs.inverted_costs_correct(2)[OF G(8)]
+
+interpretation max_version:
+  bp_min_weight_matching_algorithms_correct
+  G "curry \<Parallel>lookup (inverted_costs edge_costs)\<Parallel>" left right right_neighbs
+  using G(1-6)
+  by(auto intro!: bp_min_weight_matching_algorithms_correct.intro dest: G(7)
+        simp add: inverted_costs)
+
+lemma minus_minus_w: "- (\<lambda>e. - min_version.\<w> e) = \<w>" 
+"- (\<lambda>e. - \<Parallel>lookup edge_costs\<Parallel> \<langle>e\<rangle>) = (\<lambda>e. \<Parallel>lookup edge_costs\<Parallel> \<langle>e\<rangle>)"
+  by auto
+
+lemma compute_max_weight_perfect_matching_correct:
+"compute_max_weight_perfect_matching_inv left right edge_costs right_neighbs = None
+  \<Longrightarrow> \<nexists> M. perfect_matching G M"
+"compute_max_weight_perfect_matching_inv left right edge_costs right_neighbs = Some M
+  \<Longrightarrow> max_weight_perfect_matching G \<w> (matching_abstract M)"
+  using max_version.minimum_weight_matching_algos_correct(1,2)
+  by(auto simp add: compute_max_weight_perfect_matching_inv_def inverted_costs
+                    min_perfect_and_max_perfect_matching minus_minus_w)
+
+lemma compute_max_weight_correct:
+"max_weight_matching G \<w> (matching_abstract
+      (compute_max_weight_matching_inv left right edge_costs right_neighbs))"
+  using max_version.minimum_weight_matching_algos_correct(3)
+  by(auto simp add: compute_max_weight_matching_inv_def inverted_costs
+                    min_and_max_matching minus_minus_w)
+
+lemma compute_max_weight_max_card_correct:
+  "max_weight_max_card_matching G \<w> (matching_abstract
+      (compute_max_weight_max_card_matching_inv left right edge_costs right_neighbs))"
+  using max_version.minimum_weight_matching_algos_correct(4)
+  by(auto simp add: compute_max_weight_max_card_matching_inv_def inverted_costs
+                    min_max_card_and_max_max_card_matching  minus_minus_w)
+
+lemmas bp_weighted_matching_algos_correct =
+ min_version.minimum_weight_matching_algos_correct
+ compute_max_weight_perfect_matching_correct
+ compute_max_weight_correct
+ compute_max_weight_max_card_correct
+end
+end
